Prove lemma1, fix type class usage

history.fst
@@ -3,76 +3,65 @@ module History
 open FStar.Tactics
 module T = FStar.Tactics
 open FStar.Tactics.Typeclasses
-  
-module L = FStar.List.Tot
 
-module I = Icounter
+module L = FStar.List.Tot
 
 module M = Mrdt
 
-type state = nat
+val apply_trace : #s:eqtype -> #o:eqtype -> {| M.mrdt s o |} -> s -> t:list o -> Tot s (decreases %[t]) 
+let rec apply_trace s t =
+  match t with
+  | [] -> s
+  | op::ops -> apply_trace (M.apply_op s op) ops
 
-type history  =
- | History  : state:state
-            -> children:list (I.trace * history)
-            -> history
+type history (s:eqtype) (o:eqtype) =
+ | History  : state:s
+            -> children:list (list o * history s o)
+            -> history s o
 
-val size : h:history -> Tot nat (decreases %[h])
-val size' : l:list (I.trace * history) -> Tot nat (decreases %[l])
+val size : #s:eqtype -> #o:eqtype -> h:history s o -> Tot nat (decreases %[h])
+val size' : #s:eqtype -> #o:eqtype -> l:list (list o * history s o) -> Tot nat (decreases %[l])
 let rec size h =
     let History  _ ch = h in
     1 + size' ch
-and size'  l = 
+and size' l =
     match l with
     | [] -> 0
     | (tr,x)::xs -> size x + size' xs
 
-val hb : h1:history -> h2:history -> Tot bool (decreases (size h1))
+val hb : #s:eqtype -> #o:eqtype -> h1:history s o -> h2:history s o -> Tot bool (decreases (size h1))
 let rec hb (History s ch) h2 = 
   match ch with
   | [] -> false
   | (_,x)::xs -> x = h2 || hb x h2 || hb (History s xs) h2
 
 (* h1 --hb--> h2 <==> hbeq h1 h2 = true *)
-val hbeq : h1:history -> h2:history -> bool
+val hbeq : #s:eqtype -> #o:eqtype -> h1:history s o -> h2:history s o -> bool
 let hbeq h1 h2 = h1 = h2 || hb h1 h2
 
-val concurrent : h1:history -> h2:history -> bool
+val concurrent : #s:eqtype -> #o:eqtype -> h1:history s o -> h2:history s o -> bool
 let concurrent h1 h2 = not (hb h1 h2 || hb h2 h1 || h1 = h2)
 
-val concurrent_commutative : h1:history
-                           -> h2:history{concurrent h1 h2}
+val concurrent_commutative : #s:eqtype -> #o:eqtype 
+                           -> h1:history s o
+                           -> h2:history s o{concurrent h1 h2}
                            -> Lemma (ensures (concurrent h2 h1))
 let concurrent_commutative h1 h2 = ()
 
-val wellformed : h:history -> Tot bool (decreases h)
-val wellformed' : s:state -> l:list (I.trace * history) -> h:history -> Tot bool (decreases l)
-let rec wellformed h =
-  let History state ch = h in
-  wellformed' state ch h
-and wellformed' par_state children par_history =
-  match children with
+val wellformed : #s:eqtype -> #o:eqtype -> {| M.mrdt s o |} -> h:history s o -> Tot bool (decreases (size h))
+let rec wellformed (History s ch) =
+  match ch with
   | [] -> true
-  | (tr,x)::xs -> 
-         hb par_history x &&
-         M.apply_tr par_state tr = (History?.state x) &&
-         wellformed x &&
-         wellformed' par_state xs par_history
+  | (tr,h)::xs ->
+      apply_trace s tr = History?.state h &&
+      wellformed h &&
+      wellformed (History s xs)
 
-let _ = assert (hbeq  (History 1 [([I.Inc 1;I.Inc 1], (History 3 [([I.Inc 1],(History 4 []))]))]) (History 3 [([I.Inc 1],(History 4 []))]));()
-
-let _ = assert (hb (History 1 [([I.Inc 1;I.Inc 1], (History 3 [([I.Inc 1],(History 4 []))]))]) (History 4 []));()
-
-let _ = assert ((History 1 [([I.Inc 1;I.Inc 1], (History 3 [([I.Inc 1],(History 4 []))]))])  = (History 1 [([I.Inc 1;I.Inc 1], (History 3 [([I.Inc 1],(History 4 []))]))]));()
-
-let _ = assert (wellformed (History 1 [([I.Inc 1;I.Inc 2], (History 4 [([I.Inc 1],(History 5 []))]))]));()
-
-
-val hbeq_reflexive : h:history
-                     -> Lemma (ensures (hbeq h h))
+val hbeq_reflexive : #s:eqtype -> #o:eqtype -> h:history s o
+                   -> Lemma (ensures (hbeq h h))
 let hbeq_reflexive h = ()
 
-val lemma1 : h:history {wellformed h}
+val lemma1 : #s:eqtype -> #o:eqtype -> {| M.mrdt s o |} -> h:history s o{wellformed h}
            -> Lemma (ensures (forall h'. hbeq h h' ==> wellformed h'))  (decreases (size h))
 let rec lemma1 (History s ch) = 
   match ch with
